\documentclass[11pt]{article}

\usepackage{fullpage} 
\usepackage{hyperref}
\usepackage{amsmath}
\usepackage{amssymb}
\usepackage{amsthm}
\usepackage{graphicx}
\usepackage{pgf}
\usepackage{tikz}
\usetikzlibrary{arrows,automata}


\newcommand{\question}[2] {\vspace{0.3in}\noindent{\subsection*{Question #1. #2} \vspace{0.15in}}}

\renewcommand{\part}[1] {{\vspace{0.15in}\noindent\textbf (#1)} \vspace{0.10in}}



%  ----------------------------------------------------------------
%                         Start here
% ----------------------------------------------------------------
 
\begin{document}

\title{Assignment \#1} %Replace X with the appropriate number
\author{\Large Gustavo Estrela de Matos\\ %Replace with your name
CSCE 433: Formal Languages and Automata} %If necessary, replace with your course number and title
\date{\today}
\maketitle


\question{1}{Prove by induction that for $n \ge 1$, $\sum_{i = 1}^{n}\frac{1}{2 ^ i} = 1 - \frac{1}{2^n}$}
\begin{itemize}
\item{Base case:} For the base case we know that $n = 1$, then: \\
    $\sum_{i = 1}^{1}{\frac{1}{2^i}} = {\frac{1}{2}}$; and also $1 - {\frac{1}{2}} = {\frac{1}{2}}$.\\
    Therefore the equation holds for the base case.
\item{Inductive hypothesis:} Assume that the equation holds for $2 \leq n \leq k$ for some integer $k$\\
\item{Inductive step:} For the case where $n = k + 1$, we have that: \\
\begin{equation*}
\begin{aligned}
    \sum_{i = 1}^{k + 1}{\frac{1}{2^i}} & = \sum_{i = 1}^{k}{\frac{1}{2^i}} + {\frac{1}{2^{k + 1}}} \\
                                        & = 1 - \frac{1}{2^k} + \frac{1}{2^{k + 1}} \textup{ (by inductive hypothesis)} \\
                                        & = 1 - (\frac{1}{2^k})(1 - \frac{1}{2}) \\
                                        & = 1 - \frac{1}{2^{k + 1}} \\
\end{aligned}
\end{equation*}
    Then, if the equations holds for $k$ it also holds for $k + 1$. Now by induction, using the base case, inductive hypothesis and inductive step, we have that for all $n \geq 1$ the equation holds, as we wanted to proof.

\end{itemize}


\question{2}{Show that any integer postage greater than 7 cents can be formed by using only 3-cent and 5-cent stamps}
Basically, what we want to demonstrate is that, for any $n > 7$, $n$ can be written as 
\begin{align}
    n = 3a + 5b \label{eq2}
\end{align}
where $a$ and $b$ non negative numbers. Let $k$ be an integer such that $k > 7$ and take $k \mod 3$:
\begin{itemize}
\item{if $k \equiv 0 \mod 3$:} \\
    Then, for some integer $q \geq 0$, $k = 3q$, so equation \ref{eq2} holds.

\item{if $k \equiv 1 \mod 3$:} \\
    We have that
\begin{equation*}
\begin{aligned}
    k - 10 &\equiv 1 - 10 \mod 3\\
    k - 10 &\equiv 0 \mod 3 
\end{aligned}
\end{equation*}
    and, since $k > 7$ and $k \equiv 1 \mod 3$ we have that $k \geq 10$, hence $k - 10 \geq 0$ and there is $q \geq$ integer such that
\begin{equation*}
\begin{aligned}
    k - 10 &= 3q \\
    k      &= 3(q) + 5(2) \\
\end{aligned}
\end{equation*}
    Therefore, equation \ref{eq2} also holds for this case.

\item{if $k \equiv 2 \mod 3$:} \\
    We have that
\begin{equation*}
\begin{aligned}
    k - 5 &\equiv 2 - 5 \mod 3\\
    k - 5 &\equiv 0 \mod 3 
\end{aligned}
\end{equation*}
    and, since $k > 7$, there is $q \geq 0$ integer such that
\begin{equation*}
\begin{aligned}
    k - 5 &= 3q \\
    k &= 3(q) + 5(1) 
\end{aligned}
\end{equation*}
    Therefore, equation \ref{eq2} holds again.
\end{itemize}
Since the equation \ref{eq2} holds for all cases it holds for any case.

\question{3}{Give a DFA for each of the following languages}
\part{a} Binary strings that contais at least five 1s.\\
\part{b} Binary strings that beggins with 010 or ends with 101.\\
\part{c} Binary strings having the substring 010 but not having the substring 101. \\

\part{a}
\begin{itemize}
	\item $Q = \{q_0, q_1, q_2, q_3, q_4, q_5\}$,	
	\item $\Sigma = \{0,1\}$,
	\item $q = q_0$,
	\item $F = \{q_5\}$, and
        \item $\delta$ is defined as follows. \\

\begin{tabular}{|c||c|c|}  \hline
      & 0 & 1 \\ \hline 
      $q_0$ & $q_0$ & $q_1$ \\ \hline 
      $q_1$ & $q_1$ & $q_2$ \\ \hline
      $q_2$ & $q_2$ & $q_3$ \\ \hline
      $q_3$ & $q_3$ & $q_4$ \\ \hline 
      $q_4$ & $q_4$ & $q_5$ \\ \hline 
      $q_5$ & $q_5$ & $q_5$ \\ \hline 
\end{tabular}
\end{itemize}

\part{b}
\begin{itemize}
	\item $Q = \{q_0, q_1, q_2, q_4, q_5, q_6, q_7, q_8\}$,	
	\item $\Sigma = \{0,1\}$,
	\item $q = q_0$,
	\item $F = \{q_4, q_8\}$, and
        \item $\delta$ is defined as follows. \\

\begin{tabular}{|c||c|c|}  \hline
      & 0 & 1 \\ \hline 
      $q_0$ & $q_1$ & $q_5$ \\ \hline 
      $q_1$ & $q_7$ & $q_2$ \\ \hline
      $q_2$ & $q_4$ & $q_5$ \\ \hline
      $q_4$ & $q_4$ & $q_4$ \\ \hline 
      $q_5$ & $q_6$ & $q_5$ \\ \hline 
      $q_6$ & $q_7$ & $q_8$ \\ \hline 
      $q_7$ & $q_7$ & $q_5$ \\ \hline 
      $q_8$ & $q_6$ & $q_5$ \\ \hline 
\end{tabular}
\end{itemize}

\part{c}
\begin{itemize}
	\item $Q = \{q_0, q_1, q_2, q_3, q_4, q_5, q_6, q_7\}$,	
	\item $\Sigma = \{0,1\}$,
	\item $q = q_0$,
	\item $F = \{q_4, q_5\}$, and
        \item $\delta$ is defined as follows. \\

\begin{tabular}{|c||c|c|}  \hline
      & 0 & 1 \\ \hline 
      $q_0$ & $q_1$ & $q_2$ \\ \hline 
      $q_1$ & $q_1$ & $q_3$ \\ \hline
      $q_2$ & $q_6$ & $q_2$ \\ \hline
      $q_3$ & $q_4$ & $q_2$ \\ \hline 
      $q_4$ & $q_5$ & $q_7$ \\ \hline 
      $q_5$ & $q_5$ & $q_2$ \\ \hline 
      $q_6$ & $q_1$ & $q_7$ \\ \hline 
      $q_7$ & $q_7$ & $q_7$ \\ \hline 
\end{tabular}

\end{itemize}

\begin{figure}[h]
\centering 
\fbox{
\includegraphics{433.pdf}
}
\end{figure}

\end{document}

